coq/Progress.v
@@ -229,13 +229,6 @@ red_spec_object_delete_args_obj_4
 
 === Daniele
 
-red_stat_expr (* done *)
-red_stat_expr_1 
-
-red_stat_if (* done *)
-red_stat_if_1_true 
-red_stat_if_1_false 
-red_stat_if_1_false_implicit 
 
 red_stat_continue 
 
